wip!

Tests/STLC/Scratch.lean
@@ -1,5 +1,7 @@
 import Std
 
+namespace Tests.STLC.Scratch
+
 example : Type 1 := Type
 example : Type 1 := Type -> Type
 
@@ -11,16 +13,16 @@ inductive Box1 : (T: Type) -> Type where
 
 inductive Box3 : Type 1 where
   | mk : {T: Type} -> (v: T) -> Box3
-def Box3AlsoMk {T: Type} (v: T) : Box3 := Box3.mk v
+def box3AlsoMk {T: Type} (v: T) : Box3 := Box3.mk v
 
 inductive Box4 : Type 1 where
   | mk {T: Type} : (v: T) -> Box4
-def Box4AlsoMk {T: Type} (v: T) : Box4 := Box4.mk v
+def box4AlsoMk {T: Type} (v: T) : Box4 := Box4.mk v
 
 example : {T : Type} -> T -> Box3 := Box3.mk
-example : {T : Type} -> T -> Box3 := Box3AlsoMk
+example : {T : Type} -> T -> Box3 := box3AlsoMk
 example : {T : Type} -> T -> Box4 := Box4.mk
-example : {T : Type} -> T -> Box4 := Box4AlsoMk
+example : {T : Type} -> T -> Box4 := box4AlsoMk
 
 inductive Sys (typ: Type) (trm: Type) : Type where
 | mk : Sys typ trm
@@ -37,3 +39,5 @@ def SigmaLike (T : Type) : Type :=
 --   trm: Type
 
 -- example: Type -> Type -> Type := Sys2
+
+end Tests.STLC.Scratch
