Tests/package.lean
@@ -2,3 +2,4 @@
 import «Tests».EquivIsoDemo
 import «Tests».DOT.Sanity
 import «Tests».DTLC.package
+import «Tests».STLC.Scratch
